Save intermediate proof state on 2025-07-31

wp_proofs.sml
@@ -1,105 +1,203 @@
+(***********************************************************************)
+(* Proves about Weakest Preconditions for Pancake Statements           *)
+(*                                                                     *)
 (* These proves are based on cakeml/pancake/semantics/panSemScript.sml *)
+(***********************************************************************)
 
+(* Helper-tactic for multiple calls of Cases_on followed by gvs[], *)
+(* i.e. when eliminating non-trivial but contradictory cases       *)
+fun elim_cases []      = all_tac
+  | elim_cases (x::xs) = (Cases_on x >> gvs[] >> elim_cases xs);
+
+
+
+
+
+(***************************************************************)
+(* 1. Definitions and Theorems about Expressions as Predicates *)
+(***************************************************************)
+
+(* An expression is a predicate at a given state, if it evaluates to a ValWord *)
+Definition is_pred_def:
+  is_pred expr = λs. ∃w. eval s expr = SOME (ValWord w)
+End
+
+(* A predicate evaluates to true, if this ValWord is not zero *)
+Definition pred_eval_def:
+  pred_eval expr = λs. case (eval s expr) of
+                       | SOME (ValWord w) => w ≠ 0w
+                       | _                => F
+End
+
+(* Syntactic Lemma: A predicate evaluates to true, iff it evaluates to a non-zero value *)
+Theorem pred_eval_elem:
+  ∀s expr. s ∈ pred_eval expr ⇔ ∃w. eval s expr = SOME (ValWord w) ∧ w ≠ 0w
+Proof
+  simp[pred_eval_def]
+  >> elim_cases [‘eval s expr’, ‘x’, ‘w’]
+QED
+
+(* A predicates complement evaluates to true, if the expression is a predicate, but does not evaluate to true *)
+Definition pred_compl_def:
+  pred_compl expr = {s | s ∈ is_pred expr ∧ s ∉ pred_eval expr}
+End
+
+(* Law of excluded middle, if the expression is a predicate *)
+Theorem pred_eval_lem:
+  ∀s expr. s ∈ is_pred expr ⇒ (s ∈ pred_eval expr ∨ s ∈ pred_compl expr)
+Proof
+  rw[is_pred_def,pred_eval_def,pred_compl_def]
+QED
+
+(* Syntactic Lemma: A predicate-complement evaluates to true, iff it evaluates to a zero *)
+Theorem pred_compl_elem:
+  ∀s expr. s ∈ pred_compl expr ⇔ ∃w. eval s expr = SOME (ValWord w) ∧ w = 0w
+Proof
+  rpt strip_tac
+  >> iff_tac
+  >> rw[pred_compl_def,pred_eval_def,is_pred_def]
+  >> gvs[]
+QED
+
+
+
+
+
+(***********************************************************)
+(* 2. Definitions and Theorems about Weakest Preconditions *)
+(***********************************************************)
+
+(* A hoare triple holds, if the state being fulfilling the precondition causes termination and a state fulfilling the postcondition *)
 Definition hoare_def:
   hoare P prog Q ⇔ ∀s. s ∈ P ⇒ let (r, t) = evaluate (prog, s) in
                                r = NONE ∧ t ∈ Q
 End
 
+(* The weakest precondition is the union of all preconditions that form a hoare triple *)
 Definition wp_def:
   wp prog Q = BIGUNION {P | hoare P prog Q}
 End
 
+(* The set-based definition above implies, that is actually is the weakest precondition *)
 Theorem wp_is_weakest_precondition:
-  R = wp prog Q ⇒ (hoare R prog Q ∧ ∀P. hoare P prog Q ⇒ P ⊆ R)
+  ∀prog Q. hoare (wp prog Q) prog Q ∧ ∀P. hoare P prog Q ⇒ P ⊆ (wp prog Q)
 Proof
   rw[wp_def]
   >- (rw[hoare_def] >> gvs[])
   >- (rw[BIGUNION,SUBSET_DEF] >> qexists_tac ‘P’ >> rw[])
 QED
 
-Theorem weakest_precondition_is_wp:
-  (hoare R prog Q ∧ ∀P. hoare P prog Q ⇒ P ⊆ R) ⇒ R = wp prog Q
-Proof
-  rw[EXTENSION]
-  >> iff_tac
-  >> rw[]
-  >- (rw[wp_def] >> qexists_tac ‘R’ >> rw[])
-  >- (gvs[wp_def] >> ‘s ⊆ R’ by (rw[]) >> gvs[SUBSET_DEF])
-QED
-
-Theorem wp_causes_termination:
-  ∀s prog Q. s ∈ wp prog Q ⇒ FST (evaluate (prog, s)) = NONE
-Proof
-  rw[wp_def,hoare_def]
-  >> first_x_assum $ (drule_then assume_tac)
-  >> first_x_assum $ (fn thm => assume_tac (CONV_RULE GEN_BETA_CONV thm))
-  >> rw[]
-QED
-
-Theorem wp_causes_postcondition:
-  ∀s prog Q. s ∈ wp prog Q ⇒ SND (evaluate (prog, s)) ∈ Q
-Proof
-  rw[wp_def,hoare_def]
-  >> first_x_assum $ (drule_then assume_tac)
-  >> first_x_assum $ (fn thm => assume_tac (CONV_RULE GEN_BETA_CONV thm))
-  >> rw[]
-QED
-
+(* All preconditions are subsets of the weakest precondition *)
 Theorem all_preconditions_in_wp:
   ∀P prog Q. hoare P prog Q ⇒ P ⊆ wp prog Q
 Proof
-  rw[hoare_def,wp_def,BIGUNION,SUBSET_DEF]
-  >> qexists_tac ‘P’
-  >> rw[]
+  rw[wp_is_weakest_precondition]
 QED
 
+(* Syntactic Lemma: Therefore are the single-element preconditions also subsets of the weakest precondition *)
 Theorem all_prestates_in_wp:
   ∀x P prog Q. hoare {x} prog Q ⇒ x ∈ wp prog Q
 Proof
   rw[]
   >> assume_tac all_preconditions_in_wp
   >> first_x_assum $ (drule_then assume_tac)
-  >> gvs[SUBSET_DEF]
+  >> gvs[]
 QED
 
+(* A state is in the weakest precondition, iff it causes termination and a state fulfilling the postcondition *)
+Theorem wp_iff_postcondition:
+  ∀s prog Q. s ∈ wp prog Q ⇔ ∃t. evaluate (prog, s) = (NONE, t) ∧ t ∈ Q
+Proof
+  rpt strip_tac
+  >> iff_tac
+  >- (rw[wp_def,hoare_def]
+      >> first_x_assum $ (drule_then assume_tac)
+      >> pairarg_tac
+      >> qexists_tac ‘t’
+      >> gvs[])
+  >- (rw[]
+      >> ‘hoare {s} prog Q’ by (gvs[hoare_def])
+      >> gvs[all_prestates_in_wp])
+QED
+
+(* Is a state in the weakest precondition of an if, is the guard expression a predicate *)
+Theorem wp_if_pred_eval:
+  ∀s. s ∈ wp (If e c1 c2) Q ⇒ s ∈ is_pred e
+Proof
+  rw[]
+  >> ‘∃w. eval s e = SOME (ValWord w)’ suffices_by (rw[is_pred_def])
+  >> gvs[wp_def,hoare_def]
+  >> first_x_assum $ (drule_then assume_tac)
+  >> pairarg_tac
+  >> gvs[evaluate_def]
+  >> elim_cases [‘eval s e’, ‘x’, ‘w’]
+QED
+
+
+
+
+
+(******************************************************)
+(* 3. The Weakest Preconditions of Pancake Statements *)
+(******************************************************)
+
+(* The wp of the skip statement *)
 Theorem wp_skip:
   wp Skip Q = Q
 Proof
-  rw[wp_def,hoare_def,evaluate_def,BIGUNION,EXTENSION]
-  >> iff_tac >> rw[]
-  >- gvs[]
-  >- (qexists_tac ‘Q’ >> rw[])
+  gvs[EXTENSION,wp_iff_postcondition,evaluate_def]
 QED
 
+(* The wp of the seq statement *)
 Theorem wp_seq:
   wp p1 (wp p2 Q) = wp (Seq p1 p2) Q
 Proof
-  rw[EXTENSION,BIGUNION,wp_def]
+  rw[EXTENSION]
   >> iff_tac
   >> rw[]
-  >> qexists_tac ‘s’
-  >> gvs[hoare_def,evaluate_def]
+  >- (‘∃t. evaluate (Seq p1 p2, x) = (NONE, t) ∧ t ∈ Q’ suffices_by (metis_tac[wp_iff_postcondition])
+      >> ‘∃t. evaluate (p1, x) = (NONE, t) ∧ t ∈ wp p2 Q’ by (metis_tac[wp_iff_postcondition])
+      >> ‘∃t'. evaluate (p2, t) = (NONE, t') ∧ t' ∈ Q’ by (metis_tac[wp_iff_postcondition])
+      >> rw[evaluate_def])
+  >- (‘∃t. evaluate (p1, x) = (NONE, t) ∧ t ∈ wp p2 Q’ suffices_by (metis_tac[wp_iff_postcondition])
+      >> ‘∃t. evaluate (Seq p1 p2, x) = (NONE, t) ∧ t ∈ Q’ by (metis_tac[wp_iff_postcondition])
+      >> gvs[evaluate_def]
+      >> pairarg_tac
+      >> Cases_on ‘res’
+      >> gvs[]
+      >> ‘∃t. evaluate (p2, s1) = (NONE, t) ∧ t ∈ Q’ suffices_by (metis_tac[wp_iff_postcondition])
+      >> qexists_tac ‘t’
+      >> gvs[])
+QED
+
+(* The wp of the if statement *)
+Theorem wp_if:
+  wp (If e c1 c2) Q = (pred_eval e ∩ wp c1 Q) ∪ (pred_compl e ∩ wp c2 Q)
+Proof
+  rw[EXTENSION]
+  >> iff_tac
   >> rw[]
-  >> rpt (first_x_assum $ (drule_then assume_tac)
-          >> first_x_assum (fn thm => assume_tac (CONV_RULE GEN_BETA_CONV thm))
-          >> gvs[])
-  >> CONV_TAC GEN_BETA_CONV
-  >> rw[]
-  >- (CONV_TAC (LAND_CONV $ RAND_CONV $ GEN_BETA_CONV) >> rw[])
-  >- (CONV_TAC (LAND_CONV $ RAND_CONV $ GEN_BETA_CONV) >> rw[])
-  >> rpt (first_x_assum (fn thm => assume_tac (CONV_RULE (LAND_CONV $ RAND_CONV $ GEN_BETA_CONV) thm)))
-  >> Cases_on ‘FST (evaluate (p1,s'))’
-  >> gvs[]
-  >> qexists_tac ‘wp p2 Q’
-  >> rw[]
-  >- (CONV_TAC GEN_BETA_CONV
-      >> assume_tac wp_causes_termination
-      >> assume_tac wp_causes_postcondition
-      >> rpt (first_x_assum $ (drule_then assume_tac))
-      >> rw[])
-  >> ‘hoare {(SND (evaluate (p1,s')))} p2 Q’ suffices_by (gvs[all_prestates_in_wp])
-  >> rw[hoare_def]
-  >> CONV_TAC GEN_BETA_CONV
-  >> rw[]
+  >- (‘x ∈ is_pred e’ by (metis_tac[wp_if_pred_eval])
+      >> ‘x ∈ pred_eval e ∨ x ∈ pred_compl e’ by (metis_tac[pred_eval_lem])
+      >> gvs[Once wp_def,hoare_def,evaluate_def]
+      >> first_x_assum $ (drule_then assume_tac)
+      >- (‘x ∈ pred_eval e ∧ x ∈ wp c1 Q’ suffices_by (rw[])
+          >> ‘∃w. eval x e = SOME (ValWord w) ∧ w ≠ 0w’ by (metis_tac[pred_eval_elem])
+          >> gvs[]
+          >> ‘hoare {x} c1 Q’ by (gvs[hoare_def])
+          >> metis_tac[all_prestates_in_wp])
+      >- (‘x ∈ pred_compl e ∧ x ∈ wp c2 Q’ suffices_by (rw[])
+          >> ‘∃w. eval x e = SOME (ValWord w) ∧ w = 0w’ by (metis_tac[pred_compl_elem])
+          >> gvs[]
+          >> ‘hoare {x} c2 Q’ by (gvs[hoare_def])
+          >> metis_tac[all_prestates_in_wp]))
+  >> ‘hoare {x} (If e c1 c2) Q’ suffices_by (metis_tac[all_prestates_in_wp])
+  >> rw[hoare_def,evaluate_def]
+  >- (‘∃w. eval x e = SOME (ValWord w) ∧ w ≠ 0w’ by (metis_tac[pred_eval_elem])
+      >> ‘∃t. evaluate (c1, x) = (NONE, t) ∧ t ∈ Q’ by (metis_tac[wp_iff_postcondition])
+      >> gvs[])
+  >- (‘∃w. eval x e = SOME (ValWord w) ∧ w = 0w’ by (metis_tac[pred_compl_elem])
+      >> ‘∃t. evaluate (c2, x) = (NONE, t) ∧ t ∈ Q’ by (metis_tac[wp_iff_postcondition])
+      >> gvs[])
 QED
 
